src/tactics/FStar.Tactics.Interpreter.fs
@@ -422,6 +422,10 @@ let () =
         unify_env RE.e_env RE.e_term RE.e_term e_bool
         unify_env NRE.e_env NRE.e_term NRE.e_term NBET.e_bool;
 
+      mk_tac_step_3 0 "unify_guard_env"
+        unify_guard_env RE.e_env RE.e_term RE.e_term e_bool
+        unify_guard_env NRE.e_env NRE.e_term NRE.e_term NBET.e_bool;
+
       mk_tac_step_3 0 "match_env"
         match_env RE.e_env RE.e_term RE.e_term e_bool
         match_env NRE.e_env NRE.e_term NRE.e_term NBET.e_bool;
